Core/Metatheory/SpineType.lean
@@ -1,0 +1,19 @@
+import LeanSubst
+import Core.Term
+import Core.Term.Spine
+import Core.Reduction
+import Core.Typing
+import Core.Util
+
+import Core.Metatheory.Substitution
+import Core.Metatheory.Rename
+import Core.Metatheory.GlobalWf
+import Core.Metatheory.Uniqueness
+import Core.Metatheory.Inversion
+
+theorem SpineType.apply :
+  G&Δ, Γ ⊢ t : T ->
+  SpineType G Δ Γ sp B T ->
+  G&Δ, Γ ⊢ t.apply sp : B := by
+
+sorry
